src/coq/Handlers/OOM.v
@@ -25,64 +25,50 @@ Open Scope monad_scope.
 
 (** * Handler for out of memory
   Definition of the propositional and executable handlers for out of memory (abort).
-  - The model interpret the event as an arbitrary computation : in this model, UB can be anything, but cannot travel back in time.
-  - The interpreter simply fails.
 *)
-
-(* Technically OOM should refine OOM... *)
-Definition OOMProp (X : Type) : Type := OOM X -> Prop.
-
-Definition OOM_handler {E} : OOME ~> fun T => (OOMProp (itree E T)) :=
-  fun _ _ oomt =>
-    match oomt with
-    | Oom msg => True
-    | _ => False
-    end.
-
-Definition interp_oom_prop {E F} (h_spec : E ~> fun T => OOMProp (itree F T)) :
-  forall R (RR: relation R), itree E R -> OOMProp (itree F R).
-Admitted.
 
 Section PARAMS_MODEL.
   Variable (E F: Type -> Type).
+  Notation Effin := (E +' OOME +' F).
+  Notation Effout := (E +' OOME_NOMSG +' F).
 
-  Definition E_trigger_prop : E ~> (fun T => OOMProp (itree (E +' F) T)) :=
-    fun R e => fun oomt =>
-      match oomt with
-      | NoOom t => t = r <- trigger e ;; ret r
-      | Oom msg => True
-      end.
+  Definition E_trigger_model : E ~> itree Effout :=
+    fun R e => r <- trigger e ;; ret r.
 
-  Definition F_trigger_prop : F ~> (fun T => OOMProp (itree (E +' F) T)) :=
-    fun R e => fun oomt =>
-      match oomt with
-      | NoOom t => t = r <- trigger e ;; ret r
-      | Oom msg => True
-      end.
+  Definition F_trigger_model : F ~> itree Effout :=
+    fun R e => r <- trigger e ;; ret r.
 
-  Import PropT.
+  Definition OOM_handler : OOME ~> itree Effout
+    := fun T oome =>
+         match oome with
+         | ThrowOOM x => trigger ThrowOOM_NOMSG
+         end.
 
-  Definition model_OOM :
-    forall T (RR: T -> T -> Prop), PropT (E +' OOME +' F) T -> OOMProp (itree (E +' F) T) :=
-    fun T RR Pt (t : OOM (itree (E +' F) T)) =>
-      exists (t' : itree (E +' OOME +' F) T) , Pt t' /\ (interp_oom_prop (case_ E_trigger_prop (case_ OOM_handler F_trigger_prop)) RR t' t).
+  Definition model_OOM_h : Effin ~> itree Effout
+    := case_ E_trigger_model (case_ OOM_handler F_trigger_model).
+
+  Definition model_OOM : itree Effin ~> itree Effout
+    := interp model_OOM_h.
 
 End PARAMS_MODEL.
 
-Definition OOM_exec {E} `{FailureE -< E}: OOME ~> itree E :=
-  fun _ e => match e with | ThrowOOM s => raise ("Abort (OOM): " ++ s) end.
-
 Section PARAMS_INTERP.
   Variable (E F: Type -> Type).
+  Context `{FailureE -< F}.
+  Notation Effin := (E +' OOME +' F).
+  Notation Effout := (E +' F).
 
-  Definition E_trigger :  E ~> itree (E +' F) :=
+  Definition OOM_exec {E} `{FailureE -< E}: OOME ~> itree E :=
+    fun _ e => match e with | ThrowOOM s => raise ("Abort (OOM): " ++ s) end.
+
+  Definition E_trigger :  E ~> itree Effout :=
     fun R e => r <- trigger e ;; ret r.
 
-  Definition F_trigger : F ~> itree (E +' F) :=
+  Definition F_trigger : F ~> itree Effout :=
     fun R e => r <- trigger e ;; ret r.
 
-  Definition exec_OOM `{FailureE -< E +' F}:
-    itree (E +' OOME +' F) ~> itree (E +' F) :=
+  Definition exec_OOM :
+    itree Effin ~> itree Effout :=
     interp (case_ E_trigger (case_ OOM_exec F_trigger)).
 
 End PARAMS_INTERP.
