src/coq/Handlers/UndefinedBehaviour.v
@@ -27,18 +27,25 @@ Open Scope monad_scope.
 Definition UB_handler {E}: UBE ~> PropT E := fun _ _ _ => True.
 
 Section PARAMS_MODEL.
-  Variable (E F: Type -> Type).
+  Variable (E F G: Type -> Type).
+  Notation Effin := (E +' F +' UBE +' G).
+  Notation Effout := (E +' F +' G).
 
-  Definition E_trigger_prop : E ~> PropT (E +' F) :=
+  Definition E_trigger_prop : E ~> PropT Effout :=
     fun R e => fun t => t = r <- trigger e ;; ret r.
 
-  Definition F_trigger_prop : F ~> PropT (E +' F) :=
+  Definition F_trigger_prop : F ~> PropT Effout :=
+    fun R e => fun t => t = r <- trigger e ;; ret r.
+
+  Definition G_trigger_prop : G ~> PropT Effout :=
     fun R e => fun t => t = r <- trigger e ;; ret r.
 
   Definition model_UB :
-    forall T (RR: T -> T -> Prop), PropT (E +' UBE +' F) T -> PropT (E +' F) T :=
-    fun T RR Pt (t : itree (E +' F) T) =>
-      exists (t' : itree (E +' UBE +' F) T) , Pt t' /\ (interp_prop (case_ E_trigger_prop (case_ UB_handler F_trigger_prop)) _ RR t' t).
+    forall T (RR: T -> T -> Prop), PropT Effin T -> PropT Effout T :=
+    fun T RR Pt (t : itree Effout T) =>
+      exists (t' : itree Effin T) ,
+        Pt t' /\
+          (interp_prop (case_ E_trigger_prop (case_ F_trigger_prop (case_ UB_handler G_trigger_prop))) _ RR t' t).
 
 End PARAMS_MODEL.
 
