src/coq/Semantics/TopLevel.v
@@ -182,7 +182,7 @@ Definition interpreter_gen
            (entry : string)
            (args : list uvalue)
            (prog: list (toplevel_entity typ (block typ * list (block typ))))
-  : itree L6 res_L4 :=
+  : itree L6_exec res_L4 :=
   let t := denote_vellvm ret_typ entry args (convert_types (mcfg_of_tle prog)) in
   interp_mcfg6_exec t [] ([],[]) emptyMemState.
 
@@ -208,7 +208,7 @@ Definition model_gen
            (entry : string)
            (args : list uvalue)
            (prog: list (toplevel_entity typ (block typ * list (block typ))))
-  : OOMProp (itree L6 (MemState * (local_env * lstack * (global_env * uvalue)))) :=
+  : PropT L6 (MemState * (local_env * lstack * (global_env * uvalue))) :=
   let t := denote_vellvm ret_typ entry args (convert_types (mcfg_of_tle prog)) in
   ℑs eq t [] ([],[]) emptyMemState. 
 
